@prefix dot: <https://w3id.org/dot#> .
@prefix bot: <https://w3id.org/bot#> .
@prefix owl: <http://www.w3.org/2002/07/owl#> .
@prefix rdf: <http://www.w3.org/1999/02/22-rdf-syntax-ns#> .
@prefix xsd: <http://www.w3.org/2001/XMLSchema#> .
@prefix foaf: <http://xmlns.com/foaf/0.1/> .
@prefix rdfs: <http://www.w3.org/2000/01/rdf-schema#> .
@prefix voaf: <http://purl.org/vocommons/voaf#> .
@prefix vann: <http://purl.org/vocab/vann/> .
@prefix schema: <http://schema.org/#> .
@prefix dcterms: <http://purl.org/dc/terms/> .
@prefix seas:   <http://w3id.org/seas/> .


#################################
# METADATA
#################################

<https://github.com/Wannes-C/Thesis/blob/main/ontologyForDamageManagement.ttl> rdf:type owl:Ontology ;
    dce:modified "May 28th 2021"^^xsd:string ;
    owl:versionInfo "May 28th 2021"^^xsd:string ;
    dcterms:title "ODM: Ontology for Damage Management"@en ;
    #dcterms:description """This ontology allows for dynamically modelling damages in Linked data damage models. By means of states, occurring and resolved damages can be distinguished. It furthermore allows for organised modelling of previous damages based on when they were occurring."""@en .


#################################################################
#    Classes
#################################################################

odm:DamageState		rdf:type owl:Class ;
			rdfs:label    "Damage State"@en ;
			rdfs:comment """A damage state holds all object's occurring damages at a certain moment in time. Additional information considering these damages
				should be connected to the damages themselves. A state can furthermore hold information about properties which are altered due to these
				damages. For enabling efficient damage management, it is advised for at least providing minimal metadata regarding its time of generation
				by means of prov:generatedAtTime."""@en .

odm:CurrentDamageState	rdf:type owl:Class ;
        		rdfs:subClassOf odm:DamageState ;
        		rdfs:label      "Current Damage State"@en ;
       			rdfs:comment    """The damage state that was most recently defined. It is currently assumed to be true until actions are taken for resolving 
					damages, new damages are noticed or additional damage information is obtained. In these occasions either this state is updated 
					(remaining the current state) or a new damage state is made, becoming the current state."""@en .

odm:OutdatedDamageState	rdf:type owl:Class ;
        		rdfs:subClassOf odm:DamageState ;
        		rdfs:label      "Outdated Damage State"@en;
        		rdfs:comment    "A damage state that was true at a certain moment in the past."@en .

odm:DamagedState	rdf:type owl:Class ;
        		rdfs:subClassOf odm:DamageState ;
        		rdfs:label      "Damaged State"@en;
        		rdfs:comment    "A damage state for which the object contains one or more damages."@en .

odm:UndamagedState	rdf:type owl:Class ;
        		rdfs:subClassOf odm:DamageState ;
        		rdfs:label      "Undamaged State"@en;
        		rdfs:comment    "A damage state for which all previously occurring damages are resolved, containing no more damages"@en .


#################################################################
#    Object Properties
#################################################################

odm:hasDamageState	rdf:type owl:ObjectProperty ;
			rdfs:subPropertyOf      seas:evaluation ;
			rdfs:label    "has Damage State"@en ;
                        rdfs:comment  "Defines the relationship between an object and its damage state."@en ;
                        rdfs:range odm:DamageState .

