@prefix dot: <https://w3id.org/dot#> .
@prefix bot: <https://w3id.org/bot#> .
@prefix owl: <http://www.w3.org/2002/07/owl#> .
@prefix rdf: <http://www.w3.org/1999/02/22-rdf-syntax-ns#> .
@prefix xsd: <http://www.w3.org/2001/XMLSchema#> .
@prefix foaf: <http://xmlns.com/foaf/0.1/> .
@prefix rdfs: <http://www.w3.org/2000/01/rdf-schema#> .
@prefix voaf: <http://purl.org/vocommons/voaf#> .
@prefix vann: <http://purl.org/vocab/vann/> .
@prefix schema: <http://schema.org/#> .
@prefix dcterms: <http://purl.org/dc/terms/> .
@prefix seas:   <http://w3id.org/seas/> .


#################################
# METADATA
#################################

<https://github.com/Wannes-C/Thesis/blob/main/ontologyForDamageManagment.ttl> rdf:type owl:Ontology ;
    dce:modified "March 13th 2021"^^xsd:string ;
    owl:versionInfo "March 13th 2021"^^xsd:string ;
    dcterms:title "ODM: Ontology for Damage Management"@en ;
    #dcterms:description """  """@en .


#################################################################
#    Classes
#################################################################

odm:DamageState		rdf:type owl:Class ;
			rdfs:label    "Damage State"@en ;
			rdfs:comment """A damage state holds all object's occuring damages at a certain moment in time. Additional information considering these damages
				should be connected to the damages themselves. A state can furthermore hold information about properties which are altered due to these
				damages. For enabling efficient damage managment, it is advised for at least providing minimal metadata regarding its time of generation
				by means of prov:generatedAtTime."""@en .

opm:CurrentDamageState	rdf:type owl:Class ;
        		rdfs:subClassOf opm:DamageState ;
        		rdfs:label      "Current Damage State"@en ;
       			rdfs:comment    """The damage state that was most recently defined. It is currently assumed to be true until actions are taken for resolving 
					damages, new damages are noticed or additional damage information is obtained. In these occasions either this state is updated 
					(remaining the current state) or a new damage state is made, becoming the current state."""@en .

opm:OutdatedDamageState	rdf:type owl:Class ;
        		rdfs:subClassOf opm:DamageState ;
        		rdfs:label      "Outdated Damage State"@en;
        		rdfs:comment    "A damage state that was true at a certain moment in the past."@en .

opm:DamagedState	rdf:type owl:Class ;
        		rdfs:subClassOf opm:DamageState ;
        		rdfs:label      "Damaged State"@en;
        		rdfs:comment    "A damage state for which the object contains one or more damages."@en .

opm:UndamagedState	rdf:type owl:Class ;
        		rdfs:subClassOf opm:DamageState ;
        		rdfs:label      "Undamaged State"@en;
        		rdfs:comment    "A damage state for which all previously occuring damages are resolved, containing no more damages"@en .


#################################################################
#    Object Properties
#################################################################

odm:hasDamageState	rdf:type owl:ObjectProperty ;
			rdfs:subPropertyOf      seas:evaluation ;
			rdfs:label    "has Damage State"@en ;
                        rdfs:comment  "Defines the relationship between an object and its damage state."@en ;
                        rdfs:range odm:DamageState .

